initial work on the multiset datastructure

theories/examples/multiset.v
@@ -19,23 +19,54 @@ Definition list_match : val := λ: "ls" "f" "g",
     "g" "hd" "tl"
   end.
 
-Definition insert_high : val := λ: "ls" "v",
-  cons ("v", #true) "ls".
+Definition insert_unordered : val := λ: "ls" "v",
+  cons "v" "ls".
 
-Definition insert_low : val := rec: "insert" "ls" "v" :=
+Definition insert_ordered : val := rec: "insert" "ls" "v" :=
   list_match
     "ls"
     (λ: <>, cons "v" nil)
-    (λ: "hd" "tl", let: "sensitivity" := Snd "hd" in
-                   let: "hd" := Fst "hd" in
-                   if: "sensitivity"
-                   (* If we are still in the high security part of the list *)
-                   then "insert" "tl" "v"
-                   else if: "v" ≤ "hd"
-                        then cons ("v", #false) "ls"
-                        else "insert" "tl" "v").
+    (λ: "hd" "tl", if: "v" ≤ "hd"
+                   then cons "v" "ls"
+                   else cons "hd" ("insert" "tl" "v")).
 
-Definition size : val := λ: "ls",
+Definition insert : val := λ: "l" "v" "f",
+  let: "x" := !"l" in
+  let: "l-high" := Fst "x" in
+  let: "l-low" := Snd "x" in
+  if: "f"
+  then "l" <- (insert_unordered "l-high" "v",
+               "l-low")
+  else "l" <- ("l-high",
+               insert_ordered "l-low" "v").
+
+Definition contains_unorderd : val := rec: "contains" "ls" "v" :=
+  list_match
+    "ls"
+    (λ: <>, #false)
+    (λ: "hd" "tl", if: "v" = "hd"
+                   then #true
+                   else "contains" "tl" "v").
+
+Definition contains_ordered : val := rec: "contains" "ls" "v" :=
+  list_match
+    "ls"
+    (λ: <>, #false)
+    (λ: "hd" "tl", if: "v" = "hd"
+                   then #true
+                   else if: "hd" < "v"
+                        then #false
+                        else "contains" "tl" "v").
+
+Definition contains : val := λ: "l" "v",
+  let: "x" := !"l" in
+  let: "l-high" := Fst "x" in
+  let: "l-low" := Snd "x" in
+  if: contains_unorderd "l-high" "v"
+  then #true
+  else contains_ordered "l-low" "v".
+
+Definition size_loop : val := λ: "ls",
   let: "loop" :=
      (rec: "loop" "ls" "n" :=
           list_match
@@ -43,6 +74,12 @@ Definition size : val := λ: "ls",
             (λ: <>, "n")
             (λ: "hd" "tl", "loop" "tl" ("n"+#1))) in
   "loop" "ls" #0.
+
+Definition size : val := λ: "l",
+  let: "x" := !"l" in
+  let: "l-high" := Fst "x" in
+  let: "l-low" := Snd "x" in
+  size_loop "l-low" + size_loop "l-high".
 
 Fixpoint is_list (hd : val) (xs : list val) : Prop :=
   match xs with
@@ -62,59 +99,140 @@ Section proof.
         ⌜v1 = (w1, #b)%V⌝ ∗ ⌜v2 = (w2, #b)%V⌝ ∗
         ⟦ tint (if b then High else Low) ⟧ ξ w1 w2)%I.
 
+  Definition sec_list hd1 hd2 (l ξ : slevel) :=
+    (∃ xs1 xs2, ⌜is_list hd1 xs1⌝ ∗ ⌜is_list hd2 xs2⌝ ∗
+                 ([∗ list] v1; v2 ∈ xs1;xs2, ⟦ tint l ⟧ ξ v1 v2))%I.
+
   Definition ls_inv (l1 l2 : loc) (ξ : slevel) :=
-    (∃ hd1 hd2 (xs1 xs2 : list val), l1 ↦ₗ hd1 ∗ l2 ↦ᵣ hd2 ∗
-                        ([∗ list] v1; v2 ∈ xs1;xs2, cell_rel v1 v2 ξ) ∗
-                        ⌜is_list hd1 xs1⌝ ∗ ⌜is_list hd2 xs2⌝ ∗
-                        ⌜length xs1 = length xs2⌝)%I.
+    (∃ hdh1 hdh2 hdl1 hdl2,
+        l1 ↦ₗ (hdh1, hdl1) ∗ l2 ↦ᵣ (hdh2, hdl2) ∗
+        sec_list hdh1 hdh2 High ξ ∗
+        sec_list hdl1 hdl2 Low ξ)%I.
 
-
-  Lemma insert_high_spec l1 l2 v1 v2 ξ Φ :
-    ls_inv l1 l2 ξ -∗
-    ⟦ tint High ⟧ ξ v1 v2 -∗
-    ▷ (ls_inv l1 l2 ξ -∗ Φ #() #()) -∗
-    DWP #l1 <- insert_high !#l1 v1 &
-        #l2 <- insert_high !#l2 v2 : Φ.
+  Lemma insert_low_helper v1 v2 hd1 hd2 xs1 xs2 ξ :
+    ⟦ tint Low ⟧ ξ v1 v2 -∗
+    ([∗ list] v1; v2 ∈ xs1;xs2, ⟦ tint Low ⟧ ξ v1 v2) -∗
+    ⌜is_list hd1 xs1⌝ -∗ ⌜is_list hd2 xs2⌝ -∗
+    DWP insert_ordered hd1 v1 & insert_ordered hd2 v2
+      : λ hd1 hd2, ∃ xs1 xs2, ([∗ list] v1; v2 ∈ xs1;xs2, ⟦ tint Low ⟧ ξ v1 v2) ∗ ⌜is_list hd1 xs1⌝ ∗ ⌜is_list hd2 xs2⌝.
   Proof.
-    iDestruct 1 as (hd1 hd2 xs1 xs2) "(Hl1 & Hl2 & Hvs & #Hr)".
-    iIntros "#Hvv HΦ".
-    dwp_bind (! _)%E (! _)%E. iApply (dwp_load with "Hl1 Hl2").
-    iNext. iIntros "[Hl1 Hl2]".
-    dwp_bind (insert_high _ v1) (insert_high _ v2).
-    dwp_rec. dwp_pures. dwp_rec.
-    dwp_pures. iApply dwp_value.
-    iModIntro.
-    iApply (heap_lang_lifting.dwp_store with "Hl1 Hl2").
-    iIntros "Hl1 Hl2". iNext. iApply "HΦ".
-    iExists _,_,((v1,#true)%V::xs1),((v2,#true)%V::xs2). iFrame.
-    iSplitL.
-    { iExists _,_,true. iFrame "Hvv". eauto with iFrame. }
-    iDestruct "Hr" as %[Hxs1 [Hxs2 Hlen]].
-    repeat iSplit; iPureIntro; naive_solver.
+    iIntros "#Hvv Hvs".
+    iLöb as "IH" forall (hd1 hd2 xs1 xs2).
+    iDestruct (big_sepL2_length with "Hvs") as %Hlen.
+    iIntros "#Hr1 #Hr2".
+    iDestruct "Hr1" as %Hxs1. iDestruct "Hr2" as %Hxs2.
+    dwp_rec. dwp_pures. dwp_rec. dwp_pures.
+    destruct xs1 as [|x1 xs1'].
+    - assert (xs2 = []) as ->.
+      { destruct xs2; naive_solver. }
+      rewrite Hxs1 Hxs2.
+      dwp_pures. dwp_rec. dwp_pures.
+      iApply dwp_value. iModIntro.
+      iExists [v1],[v2].
+      iFrame "Hvv Hvs".
+      repeat iSplit; iPureIntro; try naive_solver.
+    - assert (∃ x2 xs2', xs2 = x2::xs2') as [x2 [xs2' ->]].
+      { destruct xs2; naive_solver. }
+      simpl in Hxs1, Hxs2.
+      destruct Hxs1 as [hd1' [-> Hhd1']].
+      destruct Hxs2 as [hd2' [-> Hhd2']].
+      iSimpl in "Hvs". iDestruct "Hvs" as "[H Hvs]".
+      dwp_pures.
+      (* x1 x2, v1 v2 are integers *)
+      iDestruct "H" as (? x -> ->) "H".
+      iDestruct "H" as %Hx.
+      assert (Low ⊑ ξ) as Hξ.
+      { by destruct ξ. }
+      rewrite (Hx Hξ).
+      iDestruct "Hvv" as (? v -> ->) "H".
+      iDestruct "H" as %Hv.
+      rewrite (Hv Hξ).
+      (* now we can continue symbolic execution *)
+      dwp_pures. case_bool_decide; dwp_pures.
+      + dwp_rec. dwp_pures.
+        iApply dwp_value.
+        iModIntro. iExists (#v::#x::xs1'),(#v::#x::xs2').
+        iSimpl. iFrame "Hvs". iSplitL.
+        { iSplit; iExists _,_; eauto with iFrame. }
+        iSplit; iPureIntro; naive_solver.
+      + dwp_bind (insert_ordered _ _) (insert_ordered _ _).
+        iApply (dwp_wand with "[Hvs]").
+        { iApply ("IH" with "Hvs"); iPureIntro; done. }
+        clear Hhd1' Hhd2' hd1' hd2' xs1' xs2' Hlen.
+        iIntros (hd1' hd2'). iDestruct 1 as (xs1' xs2') "[Hvs [%%]]".
+        dwp_rec. dwp_pures. iApply dwp_value.
+        iModIntro. iExists (#x::xs1'),(#x::xs2').
+        iSimpl. iFrame. iSplitL.
+        { iExists _,_; eauto with iFrame. }
+        iSplit; iPureIntro; naive_solver.
   Qed.
 
-  Lemma size_spec l1 l2 ξ Φ :
+  (* Question: can the b's here be different? *)
+  Lemma insert_spec l1 l2 v1 v2 (b : bool) ξ Φ :
     ls_inv l1 l2 ξ -∗
-    ▷ (∀ v1 v2, ⟦ tint Low ⟧ ξ v1 v2 -∗ ls_inv l1 l2 ξ -∗ Φ v1 v2) -∗
-    DWP size !#l1 & size !#l2 : Φ.
+    ⟦ tint (if b then High else Low) ⟧ ξ v1 v2 -∗
+    ▷ (ls_inv l1 l2 ξ -∗ Φ #() #()) -∗
+    DWP insert #l1 v1 #b & insert #l2 v2 #b : Φ.
   Proof.
-    iDestruct 1 as (hd1 hd2 xs1 xs2) "(Hl1 & Hl2 & Hvs & #Hr)".
-    iIntros "HΦ".
+    iDestruct 1 as (hdh1 hdh2 hdl1 hdl2) "(Hl1 & Hl2 & Hhs & Hls)".
+    iIntros "#Hvv HΦ".
+
+    dwp_rec. dwp_pures.
     dwp_bind (! _)%E (! _)%E. iApply (dwp_load with "Hl1 Hl2").
     iNext. iIntros "[Hl1 Hl2]".
-    iAssert (∀ v1 v2, ⟦ tint Low ⟧ ξ v1 v2 -∗ Φ v1 v2)%I with "[HΦ Hvs Hl1 Hl2]" as "HΦ".
-    { iIntros (v1 v2) "H". iApply ("HΦ" with "H").
-      iExists _,_,_,_. by iFrame. }
-    dwp_rec. dwp_pure _ _=>/=. dwp_pure _ _=>/=. dwp_pure _ _=>/=.
+
+    dwp_pures. destruct b; dwp_pures.
+    - (* High-security *)
+      dwp_bind (insert_unordered _ v1) (insert_unordered _ v2).
+      dwp_rec. dwp_pures. dwp_rec.
+      dwp_pures. iApply dwp_value.
+      iModIntro. dwp_pures.
+
+      iApply (heap_lang_lifting.dwp_store with "Hl1 Hl2").
+      iIntros "Hl1 Hl2". iNext.
+
+      iApply "HΦ". iExists _,_,_,_. iFrame.
+      rewrite /sec_list.
+      iDestruct "Hhs" as (xs1' xs2' Hxs1' Hxs2') "Hvs".
+      iExists (v1::xs1'), (v2::xs2'). iSimpl. iFrame "Hvs Hvv".
+      iSplit; iPureIntro; naive_solver.
+    - (* Low-security *)
+      dwp_bind (insert_ordered _ v1) (insert_ordered _ v2).
+      iApply (dwp_wand with "[Hls]").
+      { iDestruct "Hls" as (hd1 hd2 ??) "Hls".
+        iApply (insert_low_helper with "Hvv Hls [//] [//]"). }
+      iIntros (hdl1' hdl2'). iDestruct 1 as (xs1' xs2') "(Hxs & H1 & H2)".
+      dwp_pures.
+
+      iApply (heap_lang_lifting.dwp_store with "Hl1 Hl2").
+      iIntros "Hl1 Hl2". iNext.
+
+      iApply ("HΦ" with "[-]"). iExists _,_,_,_. iFrame.
+      iExists _,_. iFrame.
+  Qed.
+
+  Lemma size_helper hd1 hd2 l ξ Φ :
+    sec_list hd1 hd2 l ξ -∗
+    (∀ v1 v2, sec_list hd1 hd2 l ξ -∗ ⟦ tint Low ⟧ ξ v1 v2 -∗ Φ v1 v2) -∗
+    DWP size_loop hd1 & size_loop hd2 : Φ.
+  Proof.
+    iIntros "Hls HΦ".
+    iDestruct "Hls" as (xs1 xs2) "Hr".
+    dwp_rec.
     generalize 0. intros n. dwp_pures.
     iRevert "Hr". iLöb as "IH" forall (n hd1 hd2 xs1 xs2).
-    iIntros "#Hr". iDestruct "Hr" as %[Hxs1 [Hxs2 Hlen]].
+    iIntros "(Hxs1 & Hxs2 & Hls)".
+    iDestruct (big_sepL2_length with "Hls") as %Hlen.
+    iDestruct "Hxs1" as %Hxs1.
+    iDestruct "Hxs2" as %Hxs2.
     dwp_rec. dwp_pures.
     destruct xs1 as [|x1 xs1'].
     - assert (xs2 = []) as ->.
       { destruct xs2; naive_solver. }
       rewrite Hxs1 Hxs2.
-      dwp_pures. iApply dwp_value. iModIntro. iApply "HΦ".
+      dwp_pures. iApply dwp_value. iModIntro.
+      iApply ("HΦ" with "[-]").
+      { iExists [],[]. iFrame. iSplit; iPureIntro; naive_solver. }
       iExists n,n. eauto with iFrame.
     - assert (∃ x2 xs2', xs2 = x2::xs2') as [x2 [xs2' ->]].
       { destruct xs2; naive_solver. }
@@ -122,8 +240,61 @@ Section proof.
       destruct Hxs1 as [hd1' [-> Hhd1']].
       destruct Hxs2 as [hd2' [-> Hhd2']].
       dwp_pures.
-      iApply ("IH" $! (n+1) with "HΦ").
-      iAlways. repeat iSplit; eauto with iFrame.
+      iDestruct "Hls" as "[#Hxx Hls]".
+      iApply ("IH" $! (n+1) with "[HΦ] [-]").
+      { iIntros (v1 v2) "Hhd' Hvv".
+        iApply ("HΦ" with "[-Hvv] Hvv").
+        iDestruct "Hhd'" as (xs1 xs2) "(%&%&?)".
+        iExists (x1::xs1),(x2::xs2). iSimpl.
+        iFrame. iFrame "Hxx". iSplit; iPureIntro; naive_solver. }
+      iFrame "Hls". iSplit; iPureIntro; naive_solver.
+  Qed.
+
+  (* TODO: move to logrel/interp.v *)
+  Lemma dwp_binop e1 e2 t1 t2 l ξ :
+    (DWP e1 & e2 : ⟦ tint l ⟧ ξ) -∗
+    (DWP t1 & t2 : ⟦ tint l ⟧ ξ) -∗
+    DWP e1 + t1 & e2 + t2 : ⟦ tint l ⟧ ξ.
+  Proof.
+    iIntros "He Ht".
+    dwp_bind t1 t2. iApply (dwp_wand with "Ht").
+    iIntros (w1 w2) "Hw".
+
+    dwp_bind e1 e2. iApply (dwp_wand with "He").
+    iIntros (v1 v2) "Hv".
+
+    iDestruct "Hw" as (m1 m2 -> ->) "%".
+    iDestruct "Hv" as (n1 n2 -> ->) "%".
+    dwp_pures.
+    iApply dwp_value. iModIntro.
+    iExists _,_. iPureIntro. naive_solver.
+  Qed.
+
+  Lemma size_spec l1 l2 ξ Φ :
+    ls_inv l1 l2 ξ -∗
+    ▷ (∀ v1 v2, ⟦ tint Low ⟧ ξ v1 v2 -∗ ls_inv l1 l2 ξ -∗ Φ v1 v2) -∗
+    DWP size #l1 & size #l2 : Φ.
+  Proof.
+    iDestruct 1 as (hdh1 hdh2 hdl1 hdl2) "(Hl1 & Hl2 & Hhs & Hls)".
+    iIntros "HΦ".
+    dwp_rec.
+    dwp_bind (! _)%E (! _)%E. iApply (dwp_load with "Hl1 Hl2").
+    iNext. iIntros "[Hl1 Hl2]".
+
+    dwp_pures. dwp_bind (size_loop _) (size_loop _).
+    iApply (size_helper with "Hhs").
+    iIntros (n1 n2) "Hhs #Hn".
+
+    dwp_bind (size_loop _) (size_loop _).
+    iApply (size_helper with "Hls").
+    iIntros (m1 m2) "Hls #Hm".
+
+    iApply dwp_wand.
+    { iApply dwp_binop; iApply dwp_value; eauto with iFrame. }
+
+    iIntros (z1 z2) "Hz".
+    iApply ("HΦ" with "Hz [-]").
+    iExists _,_,_,_. by iFrame "Hl1 Hl2 Hhs Hls".
   Qed.
 
 End proof.
